src/Lean/Meta/Tactic/Grind/Arith/Cutsat/Proof.lean
@@ -37,11 +37,14 @@ partial def DvdCnstr.toExprProof (c' : DvdCnstr) : ProofM Expr := c'.caching do
     return mkApp10 (mkConst ``Int.Linear.dvd_solve_elim)
       (← getContext) (toExpr c₁.d) (toExpr c₁.p) (toExpr c₂.d) (toExpr c₂.p) (toExpr c'.d) (toExpr c'.p)
       reflBoolTrue (← c₁.toExprProof) (← c₂.toExprProof)
-  | .subst _x _c₁ _c₂ => throwError "NIY"
   | .ofEq x c =>
     return mkApp7 (mkConst ``Int.Linear.dvd_of_eq)
       (← getContext) (toExpr x) (toExpr c.p) (toExpr c'.d) (toExpr c'.p)
       reflBoolTrue (← c.toExprProof)
+  | .subst x c₁ c₂ =>
+    return mkApp10 (mkConst ``Int.Linear.eq_dvd_subst)
+      (← getContext) (toExpr x) (toExpr c₁.p) (toExpr c₂.d) (toExpr c₂.p) (toExpr c'.d) (toExpr c'.p)
+      reflBoolTrue (← c₁.toExprProof) (← c₂.toExprProof)
 
 partial def LeCnstr.toExprProof (c' : LeCnstr) : ProofM Expr := c'.caching do
   match c'.h with
@@ -59,7 +62,16 @@ partial def LeCnstr.toExprProof (c' : LeCnstr) : ProofM Expr := c'.caching do
       (← getContext) (toExpr c₁.p) (toExpr c₂.p) (toExpr c'.p)
       reflBoolTrue
       (← c₁.toExprProof) (← c₂.toExprProof)
-  | .subst _x _c₁ _c₂ => throwError "NIY"
+  | .subst x c₁ c₂ =>
+    let a := c₁.p.coeff x
+    let thm := if a ≥ 0 then
+      mkConst ``Int.Linear.eq_le_subst_nonneg
+    else
+      mkConst ``Int.Linear.eq_le_subst_nonpos
+    return mkApp8 thm
+        (← getContext) (toExpr x) (toExpr c₁.p) (toExpr c₂.p) (toExpr c'.p)
+        reflBoolTrue
+        (← c₁.toExprProof) (← c₂.toExprProof)
 
 partial def EqCnstr.toExprProof (c' : EqCnstr) : ProofM Expr := c'.caching do
   match c'.h with
@@ -67,10 +79,32 @@ partial def EqCnstr.toExprProof (c' : EqCnstr) : ProofM Expr := c'.caching do
     return h
   | .norm c =>
     return mkApp5 (mkConst ``Int.Linear.eq_norm) (← getContext) (toExpr c.p) (toExpr c'.p) reflBoolTrue (← c.toExprProof)
+  | .divCoeffs c =>
+    let k := c.p.gcdCoeffs c.p.getConst
+    return mkApp6 (mkConst ``Int.Linear.eq_coeff) (← getContext) (toExpr c.p) (toExpr c'.p) (toExpr k) reflBoolTrue (← c.toExprProof)
   | .subst x c₁ c₂  =>
     return mkApp8 (mkConst ``Int.Linear.eq_eq_subst)
       (← getContext) (toExpr x) (toExpr c₁.p) (toExpr c₂.p) (toExpr c'.p)
       reflBoolTrue (← c₁.toExprProof) (← c₂.toExprProof)
 
 end
+
+def setInconsistent (h : UnsatProof) : GoalM Unit := do
+  let hf ← withProofContext do
+    match h with
+    | .le c =>
+      trace[grind.cutsat.le.unsat] "{← c.pp}"
+      return mkApp4 (mkConst ``Int.Linear.le_unsat) (← getContext) (toExpr c.p) reflBoolTrue (← c.toExprProof)
+    | .dvd c =>
+      trace[grind.cutsat.dvd.unsat] "{← c.pp}"
+      return mkApp5 (mkConst ``Int.Linear.dvd_unsat) (← getContext) (toExpr c.d) (toExpr c.p) reflBoolTrue (← c.toExprProof)
+    | .eq c =>
+      trace[grind.cutsat.eq.unsat] "{← c.pp}"
+      if c.p.isUnsatEq then
+        return mkApp4 (mkConst ``Int.Linear.eq_unsat) (← getContext) (toExpr c.p) reflBoolTrue (← c.toExprProof)
+      else
+        let k := c.p.gcdCoeffs'
+        return mkApp5 (mkConst ``Int.Linear.eq_unsat_coeff) (← getContext) (toExpr c.p) (toExpr (Int.ofNat k)) reflBoolTrue (← c.toExprProof)
+  closeGoal hf
+
 end Lean.Meta.Grind.Arith.Cutsat
