tests/lean/run/grind_cutsat_eq_1.lean
@@ -1,5 +1,5 @@
 set_option grind.warning false
--- set_option grind.debug true -- TODO: enable after making more progress in `EqCnstr.lean`
+set_option grind.debug true
 open Int.Linear
 
 -- set_option trace.grind.cutsat.assert true
@@ -18,15 +18,42 @@ theorem ex₁ (a b : Int) (_ : 2*a + 3*b = 0) (_ : 2 ∣ 3*b + 1) : False := by
 theorem ex₂ (a b : Int) (_ : 2 ∣ 3*a + 1) (_ : 2*b + 3*a = 0) : False := by
   grind
 
-set_option trace.grind.cutsat.subst true
-
 theorem ex₃ (a b c : Int) (_ : c + 3*a = 0) (_ : 2 ∣ 3*a + 1) (_ : 2*b + c = 0) : False := by
   grind
 
 theorem ex₄ (a b c : Int) (_ : 2*c + 3*a = 0) (_ : 2*b + c = 0) (_ : 2 ∣ 3*a + 1) : False := by
   grind
 
+theorem ex₅ (a c : Int) (_ : 2*c + 3*a = 0) (_ : c + 1 = 0) : False := by
+  grind
+
+theorem ex₆ (a c : Int) (_ : c + 3*a = 0) (_ : c + 3*a = 1) : False := by
+  grind
+
+theorem ex₇ (a c : Int) (_ : c + 3*a = 0) (_ : c - 3*a = 6) (_ : 2*c + a = 0) : False := by
+  grind
+
+theorem ex₈ (a b : Int) (_ : 2 ∣ a + 1) (_ : a = 2*b) : False := by
+  grind
+
+example (a b : Int) (_ : a = 2*b) (_ : 2 ∣ a + 1) : False := by
+  grind
+
+theorem ex₉ (a b c : Int) (_ : a + 2*b = 0) (_ : -c + 2*b = 0) (_ : a + c > 1) : False := by
+  grind
+
+example (a b c : Int) (_ : a + c > 1) (_ : a + 2*b = 0) (_ : -c + 2*b = 0) : False := by
+  grind
+
+example (a b c : Int) (_ : -a + -c > 1) (_ : a + 2*b = 0) (_ : -c + 2*b = 0) : False := by
+  grind
+
 #print ex₁
 #print ex₂
 #print ex₃
 #print ex₄
+#print ex₅
+#print ex₆
+#print ex₇
+#print ex₈
+#print ex₉
